Code:

```{.haskell}
abs :: Int -> Int
abs x = let b = 0 <= x in
            if b then x else (0 - x)

test2 :: Int -> Int -> Int
test2 n m = let a = abs n
                b = abs m
                c' = b + 1
                c = a + c'
            in
              div n c
```

Constraints:

```{.haskell}
-- Γ ⊦ x:κx
-- Γ x:κx ⊦ κ1
-- Γ;x:κx ⊦ κiflet
-- Γ ⊦ n:κn
-- Γ;n:κn ⊦ m:κm
-- Γ;n:κn;m:κm ⊦ κ2
-- Γ ⊦ κlet
-- Γ;x:κx;b:{Prop v <=> 0<=x} ⊦ κif

-- Γ;x:κx;b:{Prop v <=> 0<=x} ⊦ κif <: κiflet
-- Γ;x:κx;b:{Prop v <=> 0<=x};b ⊦ {v=x} <: κif
-- Γ;x:κx;b:{Prop v <=> 0<=x};¬b ⊦ {v=0-x} <: κif
-- Γ;x:κx;b:{Prop v <=> 0<=x} ⊦ κiflet <: κ1
-- Γ ⊦ κlet <: κ2
-- Γ ⊦ κn <: κx
-- Γ;a:κ1[x := n] ⊦ κm <: κx
            -- let G = Γ;a:κ1[x := n];b:κ1[x := m];c':{v=b+1}
-- G;c:{v:Int|v=a+c'} ⊦ Int <: κlet

-- Γ;x:κx;b:{Prop v <=> 0<=x};¬b ⊦ {v=0} <: Int
-- Γ;x:κx;b:{Prop v <=> 0<=x};¬b ⊦ {v=x} <: Int
-- Γ;a:κ1[x := n];b:κ1[x := m] ⊦ {v=b} <: Int
-- Γ;a:κ1[x := n];b:κ1[x := m] ⊦ {v=1} <: Int
-- Γ;a:κ1[x := n];b:κ1[x := m];c':{v=b+1} ⊦ {v=c'} <: Int
-- Γ;a:κ1[x := n];b:κ1[x := m];c':{v=b+1} ⊦ {v=a} <: Int
-- G;c:{v:Int|v=a+c'} ⊦ κn <: Int
-- G;c:{v:Int|v=a+c'} ⊦ {v=c} <: {v:Int|¬(v=0)}
```

Starting from the only nontrivial constraint from the last set after the split, we have

```{.haskell}
-- Γ;a:κ1[x := n];b:κ1[x := m];c':{v=b+1};c:{v:Int|v=a+c'} ⊦ {v=c} <: {v:Int|¬(v=0)}
-- Γ;x:κx;b:{Prop v <=> 0<=x} ⊦ κiflet <: κ1
-- Γ;x:κx;b:{Prop v <=> 0<=x} ⊦ κif <: κiflet
-- Γ;x:κx;b:{Prop v <=> 0<=x};b ⊦ {v=x} <: κif
-- Γ;x:κx;b:{Prop v <=> 0<=x};¬b ⊦ {v=0-x} <: κif
```

This lets us build `p`:

```{.haskell}
κif: ( (b0 <=> 0<=x) /\ !b0 /\ v=0-x || (b1 <=> 0<=x) /\ b1 /\ v=x )
κiflet: (b2 <=> 0<=x) /\ κif
κ1: (b3 <=> 0<=x) /\ κiflet
κ1: (b3 <=> 0<=x) /\ (b2 <=> 0<=x) /\ ( (b0 <=> 0<=x) /\ !b0 /\ v=0-x || (b1 <=> 0<=x) /\ b1 /\ v=x )
p: (b3 <=> 0<=n) /\ (b2 <=> 0<=n) /\ ( (b0 <=> 0<=n) /\ !b0 /\ a=0-n || (b1 <=> 0<=n) /\ b1 /\ a=n ) /\ (b3 <=> 0<=m) /\ (b2 <=> 0<=m) /\ ( (b0' <=> 0<=m) /\ !b0 /\ b=0-m || (b1 <=> 0<=m) ) /\ b1 /\ b=m /\ c' = b+1 /\ c = a+c' /\ v=c |- v=0
```

as before, `p` UNSAT, so we can interpolate:

```{.haskell}
(b3 <=> 0<=n) /\ (b2 <=> 0<=n) /\ ( (b0 <=> 0<=n) /\ !b0 /\ a=0-n || (b1 <=> 0<=n) /\ b1 /\ a=n ) /\ (b3 <=> 0<=m) /\ (b2 <=> 0<=m) /\ ( (b0' <=> 0<=m) /\ !b0 /\ b=0-m || (b1 <=> 0<=m) /\ b1 /\ b=m ) /\ c' = b+1 /\ c = a+c' /\ v=c /\ v=0
true──────────┘  true──────────┘  0<=a────────────────────────────────────────────────────────────┘  0<=a──────────┘  0<=a──────────┘  0<=a/\0<=b───────────────────────────────────────────────────────┘1<=c'/\0<=a┘  1<=c─────┘  1<=c┘
```


Using the same modification as before to form 3'

```{.haskell}
abs :: Int -> Int
abs x = let b = 0 <= x in
            if b then x else (0 + x)

test2 :: Int -> Int -> Int
test2 n m = let a = abs n
                b = abs m
                c' = b + 1
                c = a + c'
            in
              div n c
```

This gives us the constraints:

```{.haskell}
-- Γ;a:κ1[x := n];b:κ1[x := m];c':{v=b+1};c:{v:Int|v=a+c'} ⊦ {v=c} <: {v:Int|¬(v=0)}
-- Γ;x:κx;b:{Prop v <=> 0<=x} ⊦ κiflet <: κ1
-- Γ;x:κx;b:{Prop v <=> 0<=x} ⊦ κif <: κiflet
-- Γ;x:κx;b:{Prop v <=> 0<=x};b ⊦ {v=x} <: κif
-- Γ;x:κx;b:{Prop v <=> 0<=x};¬b ⊦ {v=0+x} <: κif
```

as before, `p` SAT:

```{.haskell}
(b3 <=> 0<=n) /\ (b2 <=> 0<=n) /\ ( (b0 <=> 0<=n) /\ !b0 /\ a=0+n || (b1 <=> 0<=n) /\ b1 /\ a=n ) /\ (b3 <=> 0<=m) /\ (b2 <=> 0<=m) /\ ( (b0' <=> 0<=m) /\ !b0 /\ b=0+m || (b1 <=> 0<=m) /\ b1 /\ b=m ) /\ c' = b+1 /\ c = a+c' /\ v=c /\ v=0
```
